src/model.lean
@@ -41,17 +41,19 @@ def Herbrand : Type u := quotient (herbrand T)
 
 def vecterm.quo (T : theory L) (t : term L) : Herbrand T := quotient.mk' t
 
-notation `⟦`v`⟧ᵗ.`T :max := vecterm.quo T v
+notation `⟦`v`⟧ᴴ.`T :max := vecterm.quo T v
+notation `⟦`v`⟧ᴴ` :max := vecterm.quo _ v
+
 local infix ` ≋ `:80 := (@setoid.vec_r _ (herbrand T) _)
 
-instance (T : theory L) : inhabited (Herbrand T) := ⟨⟦#0⟧ᵗ.T⟩
+instance (T : theory L) : inhabited (Herbrand T) := ⟨⟦#0⟧ᴴ.T⟩
 
 namespace Herbrand
 variables {T}
 
 @[elab_as_eliminator]
 protected lemma ind_on {C : Herbrand T → Prop} (d : Herbrand T)
-  (h : ∀ t : term L, C ⟦t⟧ᵗ.T) : C d :=
+  (h : ∀ t : term L, C ⟦t⟧ᴴ.T) : C d :=
 quotient.induction_on' d h
 
 @[elab_as_eliminator, reducible]
@@ -61,7 +63,7 @@ quotient.lift_on' d f h
 
 @[simp]
 protected lemma lift_on_eq {φ} (t : term L) (f : term L → φ)
-  (h : ∀ v u, T ⊢̇ v =̇ u → f v = f u) : fopl.Herbrand.lift_on ⟦t⟧ᵗ.T f h = f t := rfl
+  (h : ∀ v u, T ⊢̇ v =̇ u → f v = f u) : fopl.Herbrand.lift_on ⟦t⟧ᴴ.T f h = f t := rfl
 
 @[elab_as_eliminator, reducible, simp]
 protected def lift_on₂ {φ} (d₁ d₂ : Herbrand T) (f : term L → term L → φ)
@@ -71,9 +73,9 @@ quotient.lift_on₂' d₁ d₂ f h
 @[simp]
 protected lemma lift_on₂_eq {φ} (t u : term L) (f : term L → term L → φ)
   (h : ∀ t₁ t₂ u₁ u₂, (T ⊢̇ t₁ =̇ u₁) → (T ⊢̇ t₂ =̇ u₂) → f t₁ t₂ = f u₁ u₂) :
-  fopl.Herbrand.lift_on₂ ⟦t⟧ᵗ.T ⟦u⟧ᵗ.T f h = f t u := rfl
+  fopl.Herbrand.lift_on₂ ⟦t⟧ᴴ.T ⟦u⟧ᴴ.T f h = f t u := rfl
 
-@[simp] lemma of_eq_of {t u : term L} : ⟦t⟧ᵗ.T = ⟦u⟧ᵗ.T ↔ (T ⊢̇ t =̇ u) :=
+lemma of_eq_of {t u : term L} : ⟦t⟧ᴴ.T = ⟦u⟧ᴴ.T ↔ (T ⊢̇ t =̇ u) :=
 by simp[vecterm.quo, vecterm.equiv, quotient.eq']
 
 @[elab_as_eliminator, reducible]
@@ -86,25 +88,64 @@ protected lemma lift_on_vec_eq {φ} {n} (u : dvector (term L) n) (f : dvector (t
   (h : ∀ (v u : dvector (term L) n), v ≋ u → f v = f u) :
 fopl.Herbrand.lift_on_vec ᵥ⟦u⟧ f h = f u := quotient.lift_on_vec_eq u f h
 
-def symbol.pconstant (c : L.pr 0) : Prop := T ⊢̇ form.const c
-
 @[simp] lemma equivs_equals : ∀ {n} (v₁ v₂ : dvector (term L) (n+1)),
   v₁ ≋ v₂ ↔ (T ⊢̇ v₁.to_vecterm ≡̇ v₂.to_vecterm)
 | 0 (t₁ :: dvector.nil) (t₂ :: dvector.nil) := by { simp, refl }
 | (n+1) (t₁ :: v₁) (t₂ :: v₂) := by { simp[equivs_equals v₁ v₂], intros, refl }
 
 def symbol.fn : ∀ {n} (f : L.fn n), dvector (Herbrand T) n → Herbrand T
-| 0     c _ := ⟦vecterm.const c⟧ᵗ.T
-| (n+1) f v := fopl.Herbrand.lift_on_vec v (λ u : dvector (term L) (n+1), ⟦vecterm.app f (u.to_vecterm)⟧ᵗ.T) 
-  $ λ v₁ v₂ eqn, by { simp at*, refine provable.e4.MP eqn }
+| 0     c _ := ⟦vecterm.const c⟧ᴴ.T
+| (n+1) f v := fopl.Herbrand.lift_on_vec v (λ u : dvector (term L) (n+1), ⟦vecterm.app f (u.to_vecterm)⟧ᴴ.T) 
+  $ λ v₁ v₂ eqn, by { simp[of_eq_of] at*, refine provable.e4.MP eqn }
+
+def function₀ (T : theory L) (c : L.fn 0) : Herbrand T := symbol.fn c dvector.nil
+
+def function₁ (T : theory L) (f : L.fn 1) (h : Herbrand T) : Herbrand T := symbol.fn f (h :: dvector.nil)
+
+def function₂ (T : theory L) (f : L.fn 2) (h₁ h₂ : Herbrand T) : Herbrand T := symbol.fn f (h₁ :: h₂ :: dvector.nil)
 
 def symbol.pr : ∀ {n} (f : L.pr n), dvector (Herbrand T) n → Prop
 | 0     c _ := T ⊢̇ form.const c
 | (n+1) p v := fopl.Herbrand.lift_on_vec v (λ u : dvector (term L) (n+1), T ⊢̇ form.app p (u.to_vecterm))
   $ λ v₁ v₂ eqn, by { simp at*, refine ⟨(provable.e5.MP eqn).MP, (provable.e5.MP (vecterm.equiv_symm _ eqn)).MP⟩  }
 
-def model (T : theory L) : model L := ⟨Herbrand T, ⟦#0⟧ᵗ.T, @symbol.fn _ T, @symbol.pr _ T⟩
+def model (T : theory L) : model L := ⟨Herbrand T, ⟦#0⟧ᴴ.T, @symbol.fn _ T, @symbol.pr _ T⟩
 notation `𝔗[`T`]` := model T
+
+protected theorem provable_iff {t₁ t₂} : T ⊢̇ t₁ =̇ t₂ ↔ ⟦t₁⟧ᴴ.T = ⟦t₂⟧ᴴ.T := by simp[of_eq_of]
+
+
+def subst₁_aux (t : term L) : Herbrand ⇑T → Herbrand T :=
+λ h, Herbrand.lift_on h (λ u, ⟦u.rew (t ^ˢ idvar)⟧ᴴ.T) $
+λ t₁ t₂ hyp, by { simp[Herbrand.of_eq_of, -provable.iff] at*, }
+
+def subst₁ : Herbrand T → Herbrand ⇑T → Herbrand T :=
+λ t h, Herbrand.lift_on t (λ t, subst₁_aux t h) $
+λ t₁ t₂ hyp, by { induction h using fopl.Herbrand.ind_on,
+  simp[subst₁_aux, Herbrand.of_eq_of, -provable.iff] at*, 
+    }
+infix ` ⊳ᴴ `:80 := subst₁
+
+@[simp] theorem const_function₀_eq {c : L.fn 0} : ⟦vecterm.const c⟧ᴴ.T = function₀ T c := rfl
+@[simp] theorem vecterm_app_function₁_eq {f : L.fn 1} {t} : ⟦vecterm.app f t⟧ᴴ.T = function₁ T f ⟦t⟧ᴴ.T := rfl 
+@[simp] theorem vecterm_app_function₂_eq {f : L.fn 2} {t₁ t₂} :
+  ⟦vecterm.app f (vecterm.cons t₁ t₂)⟧ᴴ.T = function₂ T f ⟦t₁⟧ᴴ.T ⟦t₂⟧ᴴ.T := rfl 
+
+@[simp] lemma subst₁_function₁ {h₁ : Herbrand T} {h₂ : Herbrand _} {f} :
+  h₁ ⊳ᴴ (function₁ _ f h₂) = function₁ _ f (h₁ ⊳ᴴ h₂) :=
+by { induction h₁ using fopl.Herbrand.ind_on, induction h₂ using fopl.Herbrand.ind_on,
+     rw ← vecterm_app_function₁_eq,
+     simp[-vecterm_app_function₁_eq, subst₁, Herbrand.of_eq_of], refl }
+
+@[simp] lemma subst₁_function₂ {h₁ : Herbrand T} {h₂ h₃ : Herbrand _} {f} :
+  h₁ ⊳ᴴ (function₂ _ f h₂ h₃) = function₂ _ f (h₁ ⊳ᴴ h₂) (h₁ ⊳ᴴ h₃) :=
+by { induction h₁ using fopl.Herbrand.ind_on,
+     induction h₂ using fopl.Herbrand.ind_on,
+     induction h₃ using fopl.Herbrand.ind_on,
+     rw ← vecterm_app_function₂_eq,
+     simp[-vecterm_app_function₂_eq, subst₁, Herbrand.of_eq_of], refl }
+
+
 
 end Herbrand
 
@@ -123,15 +164,16 @@ quotient (⟨form.equiv T, form_equiv_equivalence T⟩ : setoid (form L))
 
 def form.quo (T : theory L) (p : form L) : Lindenbaum T := quotient.mk' p
 
-notation `⟦`p`⟧.`T :max := form.quo T p
+notation `⟦`p`⟧ᴸ.`T :max := form.quo T p
+notation `⟦`p`⟧ᴸ` :max := form.quo _ p
 
 namespace Lindenbaum
-open provable
+open provable Herbrand
 variables {T}
 
 @[elab_as_eliminator]
 protected lemma ind_on {C : Lindenbaum T → Prop} (d : Lindenbaum T)
-  (h : ∀ p : form L, C ⟦p⟧.T) : C d :=
+  (h : ∀ p : form L, C ⟦p⟧ᴸ.T) : C d :=
 quotient.induction_on' d h
 
 @[elab_as_eliminator, reducible]
@@ -141,7 +183,7 @@ quotient.lift_on' d f h
 
 @[simp]
 protected lemma lift_on_eq {φ} (p : form L) (f : form L → φ)
-  (h : ∀ p q, T ⊢̇ p ↔̇ q → f p = f q) : fopl.Lindenbaum.lift_on ⟦p⟧.T f h = f p := rfl
+  (h : ∀ p q, T ⊢̇ p ↔̇ q → f p = f q) : fopl.Lindenbaum.lift_on ⟦p⟧ᴸ.T f h = f p := rfl
 
 @[elab_as_eliminator, reducible, simp]
 protected def lift_on₂ {φ} (d₁ d₂ : Lindenbaum T) (f : form L → form L → φ)
@@ -151,9 +193,9 @@ quotient.lift_on₂' d₁ d₂ f h
 @[simp]
 protected lemma lift_on₂_eq {φ} (p q : form L) (f : form L → form L → φ)
   (h : ∀ p₁ p₂ q₁ q₂, T ⊢̇ p₁ ↔̇ q₁ → T ⊢̇ p₂ ↔̇ q₂ → f p₁ p₂ = f q₁ q₂) :
-  fopl.Lindenbaum.lift_on₂ ⟦p⟧.T ⟦q⟧.T f h = f p q := rfl
+  fopl.Lindenbaum.lift_on₂ ⟦p⟧ᴸ.T ⟦q⟧ᴸ.T f h = f p q := rfl
 
-@[simp] lemma of_eq_of {p q : form L} : ⟦p⟧.T = ⟦q⟧.T ↔ T ⊢̇ p ↔̇ q :=
+protected lemma of_eq_of {p q : form L} : ⟦p⟧ᴸ.T = ⟦q⟧ᴸ.T ↔ T ⊢̇ p ↔̇ q :=
 by simp[form.quo, form.equiv, quotient.eq']
 
 instance : has_le (Lindenbaum T) :=
@@ -164,8 +206,8 @@ instance : has_le (Lindenbaum T) :=
 instance : has_lt (Lindenbaum T) := ⟨λ l k, l ≤ k ∧ ¬k ≤ l⟩
 
 def imply : Lindenbaum T → Lindenbaum T → Lindenbaum T :=
-λ p₁ p₂, Lindenbaum.lift_on₂ p₁ p₂ (λ p₁ p₂, ⟦p₁ →̇ p₂⟧.T) $
- λ p₁ p₂ q₁ q₂ hp hq, by { simp at*, split,
+λ p₁ p₂, Lindenbaum.lift_on₂ p₁ p₂ (λ p₁ p₂, ⟦p₁ →̇ p₂⟧ᴸ.T) $
+ λ p₁ p₂ q₁ q₂ hp hq, by { simp[Lindenbaum.of_eq_of] at*, split,
    { refine provable.deduction.mp (provable.deduction.mp _),
      have : T+{p₁ →̇ p₂}+{q₁} ⊢̇ p₁, from (show _ ⊢̇ q₁ →̇ p₁, by simp[hp]).MP (by simp),
      have : T+{p₁ →̇ p₂}+{q₁} ⊢̇ p₂, from (show _ ⊢̇ p₁ →̇ p₂, by simp).MP this,
@@ -174,11 +216,11 @@ def imply : Lindenbaum T → Lindenbaum T → Lindenbaum T :=
      have : T+{q₁ →̇ q₂}+{p₁} ⊢̇ q₁, from (show _ ⊢̇ p₁ →̇ q₁, by simp[hp]).MP (by simp),
      have : T+{q₁ →̇ q₂}+{p₁} ⊢̇ q₂, from (show _ ⊢̇ q₁ →̇ q₂, by simp).MP this,
      exact (show _ ⊢̇ q₂ →̇ p₂, by simp[hq]).MP this  } }
-infixr ` ⊳ `:60 := imply
+infixr ` ⊑ `:60 := imply
 
-instance : has_mul (Lindenbaum T) :=
-⟨λ p₁ p₂, Lindenbaum.lift_on₂ p₁ p₂ (λ p₁ p₂, ⟦p₁ ⩑ p₂⟧.T) $
- λ p₁ p₂ q₁ q₂ hp hq, by { simp at*, split,
+instance : has_inf (Lindenbaum T) :=
+⟨λ p₁ p₂, Lindenbaum.lift_on₂ p₁ p₂ (λ p₁ p₂, ⟦p₁ ⩑ p₂⟧ᴸ.T) $
+ λ p₁ p₂ q₁ q₂ hp hq, by { simp[Lindenbaum.of_eq_of] at*, split,
    { apply provable.deduction.mp,
      have : T+{p₁ ⩑ p₂} ⊢̇ p₁ ⩑ p₂, from provable.add _ _, simp at *,
      refine ⟨(show T+{p₁ ⩑ p₂} ⊢̇ p₁ →̇ q₁, by simp[hp]).MP this.1,
@@ -188,24 +230,24 @@ instance : has_mul (Lindenbaum T) :=
      refine ⟨(show T+{q₁ ⩑ q₂} ⊢̇ q₁ →̇ p₁, by simp[hp]).MP this.1,
        (show T+{q₁ ⩑ q₂} ⊢̇ q₂ →̇ p₂, by simp[hq]).MP this.2⟩ } }⟩
 
-instance : has_add (Lindenbaum T) :=
-⟨λ p₁ p₂, Lindenbaum.lift_on₂ p₁ p₂ (λ p₁ p₂, ⟦p₁ ⩒ p₂⟧.T) $
- λ p₁ p₂ q₁ q₂ hp hq, by { simp at*, split,
+instance : has_sup (Lindenbaum T) :=
+⟨λ p₁ p₂, Lindenbaum.lift_on₂ p₁ p₂ (λ p₁ p₂, ⟦p₁ ⩒ p₂⟧ᴸ.T) $
+ λ p₁ p₂ q₁ q₂ hp hq, by { simp[Lindenbaum.of_eq_of] at*, split,
    { refine (provable.deduction.mp ((provable.or_l _ _).MP (provable.deduction.mpr hp.1))).hyp_or
        (provable.deduction.mp ((provable.or_r _ _).MP (provable.deduction.mpr hq.1))) },
    { refine (provable.deduction.mp ((provable.or_l _ _).MP (provable.deduction.mpr hp.2))).hyp_or
        (provable.deduction.mp ((provable.or_r _ _).MP (provable.deduction.mpr hq.2))) }  }⟩
 
-instance : has_inv (Lindenbaum T) :=
-⟨λ p, Lindenbaum.lift_on p (λ p, ⟦¬̇p⟧.T) $
- λ p₁ p₂ hyp, by { simp[provable.contrapose] at*, refine ⟨hyp.2, hyp.1⟩ }⟩
+instance : has_compl (Lindenbaum T) :=
+⟨λ p, Lindenbaum.lift_on p (λ p, ⟦¬̇p⟧ᴸ.T) $
+ λ p₁ p₂ hyp, by { simp[provable.contrapose, Lindenbaum.of_eq_of] at*, refine ⟨hyp.2, hyp.1⟩ }⟩
 
-instance : has_one (Lindenbaum T) := ⟨⟦⊤̇⟧.T⟩
+instance : has_top (Lindenbaum T) := ⟨⟦⊤̇⟧ᴸ.T⟩
 
-instance : has_zero (Lindenbaum T) := ⟨⟦⊥̇⟧.T⟩
+instance : has_bot (Lindenbaum T) := ⟨⟦⊥̇⟧ᴸ.T⟩
 
-def fal : Lindenbaum ⇑T → Lindenbaum T := λ p, Lindenbaum.lift_on p (λ p, ⟦Ȧp⟧.T) $
-λ p₁ p₂ hyp, by { simp at*, 
+def fal : Lindenbaum ⇑T → Lindenbaum T := λ p, Lindenbaum.lift_on p (λ p, ⟦Ȧp⟧ᴸ.T) $
+λ p₁ p₂ hyp, by { simp[Lindenbaum.of_eq_of] at*, 
   suffices : ∀ {q₁ q₂}, ⇑T ⊢̇ q₁ →̇ q₂ → T ⊢̇ Ȧq₁ →̇ Ȧq₂, { refine ⟨this hyp.1, this hyp.2⟩ },
   intros q₁ q₂ hyp,
   refine provable.deduction.mp (provable.GE _),
@@ -214,8 +256,8 @@ def fal : Lindenbaum ⇑T → Lindenbaum T := λ p, Lindenbaum.lift_on p (λ p, 
     exact lmm₂.MP lmm₁ }
 prefix `∏`:90 := fal
 
-def ex : Lindenbaum ⇑T → Lindenbaum T := λ p, Lindenbaum.lift_on p (λ p, ⟦Ėp⟧.T) $
-λ p₁ p₂ hyp, by { simp[form.ex, provable.contrapose] at*, 
+def ex : Lindenbaum ⇑T → Lindenbaum T := λ p, Lindenbaum.lift_on p (λ p, ⟦Ėp⟧ᴸ.T) $
+λ p₁ p₂ hyp, by { simp[form.ex, provable.contrapose, Lindenbaum.of_eq_of] at*, 
   suffices : ∀ {q₁ q₂}, ⇑T ⊢̇ q₁ →̇ q₂ → T ⊢̇ Ȧ¬̇q₂ →̇ Ȧ¬̇q₁, { refine ⟨this hyp.1, this hyp.2⟩ },
   intros q₁ q₂ hyp,
   refine provable.deduction.mp (provable.GE _),
@@ -226,17 +268,17 @@ def ex : Lindenbaum ⇑T → Lindenbaum T := λ p, Lindenbaum.lift_on p (λ p, �
 prefix `∐`:90 := ex
 
 @[simp] def predicate : ∀ {n} (f : L.pr n), dvector (Herbrand T) n → Lindenbaum T
-| 0     c _ := ⟦form.const c⟧.T
-| (n+1) p v := fopl.Herbrand.lift_on_vec v (λ u : dvector (term L) (n+1), ⟦form.app p (u.to_vecterm)⟧.T)
-  $ λ v₁ v₂ eqn, by { simp at*, refine ⟨provable.e5.MP eqn, provable.e5.MP (vecterm.equiv_symm _ eqn)⟩ }
+| 0     c _ := ⟦form.const c⟧ᴸ.T
+| (n+1) p v := fopl.Herbrand.lift_on_vec v (λ u : dvector (term L) (n+1), ⟦form.app p (u.to_vecterm)⟧ᴸ.T)
+  $ λ v₁ v₂ eqn, by { simp[Lindenbaum.of_eq_of] at*, refine ⟨provable.e5.MP eqn, provable.e5.MP (vecterm.equiv_symm _ eqn)⟩ }
 
-def predicate₁ (f : L.pr 1) (h : Herbrand T) : Lindenbaum T := predicate f (h :: dvector.nil)
+def predicate₁ (T : theory L) (f : L.pr 1) (h : Herbrand T) : Lindenbaum T := predicate f (h :: dvector.nil)
 
-def predicate₂ (f : L.pr 2) (h₁ h₂ : Herbrand T) : Lindenbaum T := predicate f (h₁ :: h₂ :: dvector.nil)
+def predicate₂ (T : theory L) (f : L.pr 2) (h₁ h₂ : Herbrand T) : Lindenbaum T := predicate f (h₁ :: h₂ :: dvector.nil)
 
 def equal : Herbrand T → Herbrand T → Lindenbaum T :=
-λ h₁ h₂, fopl.Herbrand.lift_on₂ h₁ h₂ (λ t₁ t₂, ⟦t₁ =̇ t₂⟧.T) $
-λ t₁ t₂ u₁ u₂ eqn₁ eqn₂, by { simp, refine ⟨provable.deduction.mp _, provable.deduction.mp  _⟩,
+λ h₁ h₂, fopl.Herbrand.lift_on₂ h₁ h₂ (λ t₁ t₂, ⟦t₁ =̇ t₂⟧ᴸ.T) $
+λ t₁ t₂ u₁ u₂ eqn₁ eqn₂, by { simp[Lindenbaum.of_eq_of], refine ⟨provable.deduction.mp _, provable.deduction.mp  _⟩,
   have lmm₁ : T+{t₁ =̇ t₂} ⊢̇ u₁ =̇ t₁, simp [provable.e2.MP eqn₁],
   have lmm₂ : T+{t₁ =̇ t₂} ⊢̇ t₁ =̇ t₂, simp,
   have lmm₃ : T+{t₁ =̇ t₂} ⊢̇ t₂ =̇ u₂, simp [eqn₂],
@@ -247,117 +289,177 @@ def equal : Herbrand T → Herbrand T → Lindenbaum T :=
   refine (lmm₁.eq_trans lmm₂).eq_trans lmm₃ }
 infix ` ⋈ `:80 := equal
 
+def subst₁_aux (t : term L) : Lindenbaum ⇑T → Lindenbaum T :=
+λ p, Lindenbaum.lift_on p (λ p, ⟦p.subst₁ t⟧ᴸ.T) $
+λ p₁ p₂ hyp, by { simp[Lindenbaum.of_eq_of, -provable.iff] at*,
+   have := (GE hyp).subst₁ t, simp[form.subst₁, -provable.iff] at this, refine this }
+
+def subst₁ : Herbrand T → Lindenbaum ⇑T → Lindenbaum T :=
+λ t l, Herbrand.lift_on t (λ t, subst₁_aux t l) $
+λ t₁ t₂ hyp, by { induction l using fopl.Lindenbaum.ind_on,
+  simp[subst₁_aux, Lindenbaum.of_eq_of, -provable.iff] at*, 
+    }
+
+infix ` ⊳ `:80 := subst₁
+
 def sf : Lindenbaum T → Lindenbaum ⇑T := λ p, Lindenbaum.lift_on p (λ p, ⟦p.sf⟧.⇑T) $
 λ p₁ p₂ hyp, by { simp[form.ex, provable.contrapose] at*, have := provable.dummy_fal_quantifir_iff, }
 
-def provable : Lindenbaum T → Prop := λ p, Lindenbaum.lift_on p (λ p, T ⊢̇ p) $
+def Box : Lindenbaum T → Prop := λ p, Lindenbaum.lift_on p (λ p, T ⊢̇ p) $
 λ p₁ p₂ hyp, by { simp at*, refine ⟨λ h, hyp.1.MP h, λ h, hyp.2.MP h⟩ }
-prefix `□`:80 := provable
+prefix `□`:80 := Box
 
-def refutable : Lindenbaum T → Prop := λ p, ¬□p⁻¹
+def refutable : Lindenbaum T → Prop := λ p, ¬□pᶜ
 prefix `◇`:80 := refutable
 
 lemma le_antisymm {l k : Lindenbaum T} : l ≤ k → k ≤ l → l = k :=
 begin
   induction l using fopl.Lindenbaum.ind_on,
   induction k using fopl.Lindenbaum.ind_on,
-  simp[has_le.le], refine λ h₁ h₂, ⟨h₁, h₂⟩
+  simp[has_le.le, Lindenbaum.of_eq_of], refine λ h₁ h₂, ⟨h₁, h₂⟩
 end
+lemma Box_iff {l : Lindenbaum T} : ⊤ ≤ l ↔ □l :=
+by { induction l using fopl.Lindenbaum.ind_on, simp[has_top.top, Box, has_le.le] }
 
-lemma imply_le {l k : Lindenbaum T} : l ⊳ k = 1 ↔ l ≤ k :=
+lemma imply_le {l k : Lindenbaum T} : l ⊑ k = ⊤ ↔ l ≤ k := by sorry
 
+lemma provable_GE {l : Lindenbaum ⇑T} : ⊤ ≤ l → ⊤ ≤ ∏l :=
+by { simp[Box_iff], induction l using fopl.Lindenbaum.ind_on, simp[fal, Box], exact provable.GE }
 
-lemma provable_GE {l : Lindenbaum ⇑T} : □l → □∏l :=
-by { induction l using fopl.Lindenbaum.ind_on, simp[fal, provable], exact provable.GE }
+lemma provable_AX {p} (h : p ∈ T) : ⟦p⟧ᴸ.T = ⊤ :=
+by simp[has_top.top, provable.AX h, Lindenbaum.of_eq_of]
 
-lemma provable_AX {p} (h : p ∈ T) : ⟦p⟧.T = 1 :=
-by simp[has_one.one, provable.AX h]
-
-lemma provable_K {l k : Lindenbaum T} : □(l ⊳ k) → □l → □k :=
+lemma provable_K {l k : Lindenbaum T} : □(l ⊑ k) → □l → □k :=
 begin
   induction l using fopl.Lindenbaum.ind_on,
   induction k using fopl.Lindenbaum.ind_on,
-  simp[imply, provable], refine λ h₁ h₂, h₁.MP h₂
+  simp[imply, Box], refine λ h₁ h₂, h₁.MP h₂
 end
 
-@[simp] lemma equal_refl {h : Herbrand T}  : h ⋈ h = 1 :=
-by induction h using fopl.Herbrand.ind_on; simp[equal, has_one.one]
+@[simp] lemma equal_refl {h : Herbrand T}  : h ⋈ h = ⊤ :=
+by induction h using fopl.Herbrand.ind_on; simp[equal, has_top.top, Lindenbaum.of_eq_of]
 
-@[simp] lemma equal_subst₁ {h₁ h₂ : Herbrand T} {p : L.pr 1} : h₁ ⋈ h₂ ≤ predicate₁ p h₁ ⊳ predicate₁ p h₂ :=
+lemma equal_iff {h₁ h₂ : Herbrand T} {p : L.pr 1} : ⊤ ≤ h₁ ⋈ h₂ ↔ h₁ = h₂ :=
+by { simp[Box_iff], induction h₁ using fopl.Herbrand.ind_on, induction h₂ using fopl.Herbrand.ind_on,
+      simp[Lindenbaum.of_eq_of, equal, has_le.le, imply, has_top.top, Box, predicate₁,
+        (show ⟦h₁⟧ᴴ.T :: dvector.nil = ᵥ⟦h₁ :: dvector.nil⟧, by refl),
+        (show ⟦h₂⟧ᴴ.T :: dvector.nil = ᵥ⟦h₂ :: dvector.nil⟧, by refl) ], exact iff.symm Herbrand.of_eq_of }
+
+@[simp] lemma equal_subst_pr₁ {h₁ h₂ : Herbrand T} {p : L.pr 1} :
+  h₁ ⋈ h₂ ≤ predicate₁ _ p h₁ ⊑ predicate₁ _ p h₂ :=
 by { induction h₁ using fopl.Herbrand.ind_on, induction h₂ using fopl.Herbrand.ind_on,
-      simp[equal, has_le.le, imply, has_one.one, predicate₁,
-        (show ⟦h₁⟧ᵗ.T :: dvector.nil = ᵥ⟦h₁ :: dvector.nil⟧, by refl),
-        (show ⟦h₂⟧ᵗ.T :: dvector.nil = ᵥ⟦h₂ :: dvector.nil⟧, by refl) ], 
-        }
+      simp[equal, has_le.le, imply, has_top.top, predicate₁,
+        (show ⟦h₁⟧ᴴ.T :: dvector.nil = ᵥ⟦h₁ :: dvector.nil⟧, by refl),
+        (show ⟦h₂⟧ᴴ.T :: dvector.nil = ᵥ⟦h₂ :: dvector.nil⟧, by refl) ],
+        refine @provable.e5 _ T _ h₁ h₂ p }
 
-lemma double_inv (l : Lindenbaum T) : l⁻¹⁻¹ = l :=
-by induction l using fopl.Lindenbaum.ind_on; simp[has_inv.inv]
+@[simp] lemma equal_subst_fn₁ {h₁ h₂ : Herbrand T} {f : L.fn 1} : 
+  h₁ ⋈ h₂ ≤ function₁ _ f h₁ ⋈ function₁ _ f h₂ :=
+by { induction h₁ using fopl.Herbrand.ind_on, induction h₂ using fopl.Herbrand.ind_on,
+      simp[equal, has_le.le, imply, has_top.top, Herbrand.function₁,
+        (show ⟦h₁⟧ᴴ.T :: dvector.nil = ᵥ⟦h₁ :: dvector.nil⟧, by refl),
+        (show ⟦h₂⟧ᴴ.T :: dvector.nil = ᵥ⟦h₂ :: dvector.nil⟧, by refl) ],
+        refine @provable.e4 _ T _ h₁ h₂ f }
+
+@[simp] lemma double_inv (l : Lindenbaum T) : lᶜᶜ = l :=
+by induction l using fopl.Lindenbaum.ind_on; simp[Lindenbaum.of_eq_of, has_compl.compl]
 
 #check provable.prenex_fal_quantifir_imp1 _ _
 
-lemma prenex_fal_quantifir_imp1  {l : Lindenbaum ⇑T} {k : Lindenbaum T} : ∏l ⊳ k = ∐(l ⊳ k.sf) := by sorry
+lemma prenex_fal_quantifir_imp1  {l : Lindenbaum ⇑T} {k : Lindenbaum T} : ∏l ⊑ k = ∐(l ⊑ k.sf) := by sorry
 
-lemma prenex_fal_quantifir_neg  {l : Lindenbaum ⇑T} : (∏l)⁻¹ = ∐l⁻¹  := by sorry
+lemma prenex_fal_quantifir_neg  {l : Lindenbaum ⇑T} : (∏l)ᶜ = ∐lᶜ  := by sorry
 
-@[simp] lemma provable_one : □(1 : Lindenbaum T) :=
-by simp[has_one.one, provable]
+lemma subst₁_le_ex (l : Lindenbaum ⇑T) (h) : h ⊳ l ≤ ∐l :=
+begin
+  induction l using fopl.Lindenbaum.ind_on, 
+  induction h using fopl.Herbrand.ind_on, 
+  simp[ex, has_le.le, subst₁, subst₁_aux],
+  apply contrapose.mp, simp[form.ex],
+  rw (show ¬̇(l.subst₁ h) = (¬̇l).subst₁ h, by simp[form.subst₁, form.rew]), 
+  exact provable.q1
+end
 
-@[simp] lemma one_maximum (l : Lindenbaum T) : l ≤ 1 :=
-by induction l using fopl.Lindenbaum.ind_on; simp[has_one.one, has_le.le]
+@[simp] lemma subst₁_and {h : Herbrand _} {l m : Lindenbaum ⇑T} : h ⊳ (l ⊓ m) = h ⊳ l ⊓ h ⊳ m :=
+by { induction l using fopl.Lindenbaum.ind_on, induction m using fopl.Lindenbaum.ind_on, 
+     induction h using fopl.Herbrand.ind_on,
+     simp[has_inf.inf, has_le.le, subst₁, subst₁_aux, Lindenbaum.of_eq_of] }
 
-@[simp] lemma zero_minimum (l : Lindenbaum T) : 0 ≤ l :=
-by induction l using fopl.Lindenbaum.ind_on; simp[has_zero.zero, has_le.le]
+@[simp] lemma subst₁_or {h : Herbrand _} {l m : Lindenbaum ⇑T} : h ⊳ (l ⊔ m) = h ⊳ l ⊔ h ⊳ m :=
+by { induction l using fopl.Lindenbaum.ind_on, induction m using fopl.Lindenbaum.ind_on, 
+     induction h using fopl.Herbrand.ind_on,
+     simp[has_sup.sup, has_le.le, subst₁, subst₁_aux, Lindenbaum.of_eq_of] }
 
-lemma Box_iff {l : Lindenbaum T} : □l ↔ l = 1 :=
-by { split, 
-     { induction l using fopl.Lindenbaum.ind_on, simp[has_one.one, provable], intros hyp_l,
-       refine provable.deduction.mp (provable.weakening hyp_l _) },
-     { intros h, simp[h] } }
-
-lemma mul_le_l {l k : Lindenbaum T} : l * k ≤ l :=
-by { induction l using fopl.Lindenbaum.ind_on, induction k using fopl.Lindenbaum.ind_on,
-     simp[has_mul.mul, has_le.le], refine provable.deduction.mp _, have := provable.add T (l ⩑ k), simp* at * }
-
-lemma mul_le_r {l k : Lindenbaum T} : l * k ≤ k :=
-by { induction l using fopl.Lindenbaum.ind_on, induction k using fopl.Lindenbaum.ind_on,
-     simp[has_mul.mul, has_le.le], refine provable.deduction.mp _, have := provable.add T (l ⩑ k), simp* at * }
-
-lemma add_le_l {l k : Lindenbaum T} : l ≤ l + k :=
-by { induction l using fopl.Lindenbaum.ind_on, induction k using fopl.Lindenbaum.ind_on,
-     simp[has_add.add, has_le.le, provable.or_l] }
-
-lemma add_le_r {l k : Lindenbaum T} : k ≤ l + k :=
-by { induction l using fopl.Lindenbaum.ind_on, induction k using fopl.Lindenbaum.ind_on,
-     simp[has_add.add, has_le.le, provable.or_r] }
-
-private lemma sup_le {l m n : Lindenbaum T} : l ≤ n → m ≤ n → l + m ≤ n :=
+@[simp] lemma subst₁_neg {h : Herbrand _} {l : Lindenbaum ⇑T} : h ⊳ lᶜ = (h ⊳ l)ᶜ :=
 by { induction l using fopl.Lindenbaum.ind_on,
-       induction m using fopl.Lindenbaum.ind_on,
-       induction n using fopl.Lindenbaum.ind_on, simp[has_le.le, has_add.add],
-       intros h₁ h₂, exact provable.hyp_or h₁ h₂   }
+     induction h using fopl.Herbrand.ind_on,
+     simp[has_compl.compl, has_le.le, subst₁, subst₁_aux, Lindenbaum.of_eq_of] }
 
-private lemma le_inf {l m n : Lindenbaum T} : l ≤ m → l ≤ n → l ≤ m * n :=
+@[simp] lemma subst₁_equal (h₁ : Herbrand T) {h₂ h₃ : Herbrand ⇑T} :
+  h₁ ⊳ (h₂ ⋈ h₃) = (h₁ ⊳ᴴ h₂) ⋈ (h₁ ⊳ᴴ h₃) :=
+by { induction h₁ using fopl.Herbrand.ind_on, induction h₂ using fopl.Herbrand.ind_on,
+     induction h₃ using fopl.Herbrand.ind_on,
+     simp[equal, subst₁, Herbrand.subst₁, Herbrand.subst₁_aux, subst₁_aux, Lindenbaum.of_eq_of],
+     split, 
+      }
+
+@[simp] lemma provable_one : □(⊤ : Lindenbaum T) :=
+by simp[has_top.top, Box]
+
+@[simp] lemma one_maximum (l : Lindenbaum T) : l ≤ ⊤ :=
+by induction l using fopl.Lindenbaum.ind_on; simp[has_top.top, has_le.le]
+
+@[simp] lemma zero_minimum (l : Lindenbaum T) : ⊥ ≤ l :=
+by induction l using fopl.Lindenbaum.ind_on; simp[has_bot.bot, has_le.le]
+
+lemma mul_le_l (l k : Lindenbaum T) : l ⊓ k ≤ l :=
+by { induction l using fopl.Lindenbaum.ind_on, induction k using fopl.Lindenbaum.ind_on,
+     simp[has_inf.inf, has_le.le], refine provable.deduction.mp _, have := provable.add T (l ⩑ k), simp* at * }
+
+lemma mul_le_r (l k : Lindenbaum T) : l ⊓ k ≤ k :=
+by { induction l using fopl.Lindenbaum.ind_on, induction k using fopl.Lindenbaum.ind_on,
+     simp[has_inf.inf, has_le.le], refine provable.deduction.mp _, have := provable.add T (l ⩑ k), simp* at * }
+
+lemma add_le_l (l k : Lindenbaum T) : l ≤ l ⊔ k :=
+by { induction l using fopl.Lindenbaum.ind_on, induction k using fopl.Lindenbaum.ind_on,
+     simp[has_sup.sup, has_le.le, provable.or_l] }
+
+lemma add_le_r (l k : Lindenbaum T) : k ≤ l ⊔ k :=
+by { induction l using fopl.Lindenbaum.ind_on, induction k using fopl.Lindenbaum.ind_on,
+     simp[has_sup.sup, has_le.le, provable.or_r] }
+
+private lemma le_trans {l m n : Lindenbaum T} : l ≤ m → m ≤ n → l ≤ n :=
+by { induction l using fopl.Lindenbaum.ind_on,
+     induction m using fopl.Lindenbaum.ind_on,
+     induction n using fopl.Lindenbaum.ind_on, simp[has_le.le], refine provable.imp_trans }
+
+private lemma sup_le {l m n : Lindenbaum T} : l ≤ n → m ≤ n → l ⊔ m ≤ n :=
+by { induction l using fopl.Lindenbaum.ind_on,
+     induction m using fopl.Lindenbaum.ind_on,
+     induction n using fopl.Lindenbaum.ind_on, simp[has_le.le, has_sup.sup],
+     intros h₁ h₂, exact provable.hyp_or h₁ h₂   }
+
+private lemma le_inf {l m n : Lindenbaum T} : l ≤ m → l ≤ n → l ≤ m ⊓ n :=
 by { induction l using fopl.Lindenbaum.ind_on,
      induction m using fopl.Lindenbaum.ind_on,
      induction n using fopl.Lindenbaum.ind_on,
-     simp[has_le.le, has_mul.mul],
+     simp[has_le.le, has_inf.inf],
      refine λ h₁ h₂, provable.deduction.mp _, simp,
      refine ⟨provable.deduction.mpr h₁, provable.deduction.mpr h₂⟩  }
 
-private lemma le_sup_inf {l m n : Lindenbaum T} : (l + m) * (l + n) ≤ l + m * n :=
+private lemma le_sup_inf {l m n : Lindenbaum T} : (l ⊔ m) ⊓ (l ⊔ n) ≤ l ⊔ m ⊓ n :=
 by { induction l using fopl.Lindenbaum.ind_on,
      induction m using fopl.Lindenbaum.ind_on,
      induction n using fopl.Lindenbaum.ind_on,
-     simp[has_add.add, has_mul.mul, has_le.le, provable.or_r, form.or],
+     simp[has_sup.sup, has_inf.inf, has_le.le, provable.or_r, form.or],
      refine provable.deduction.mp (provable.deduction.mp _),
      have lmm₁ : T+{(¬̇l →̇ m) ⩑ (¬̇l →̇ n)}+{¬̇l} ⊢̇ (¬̇l →̇ m) ⩑ (¬̇l →̇ n), simp[-provable.and],
      have lmm₂ : T+{(¬̇l →̇ m) ⩑ (¬̇l →̇ n)}+{¬̇l} ⊢̇ ¬̇l, simp,
      simp at lmm₁ ⊢, refine ⟨lmm₁.1.MP lmm₂, lmm₁.2.MP lmm₂⟩ }
 
-
-private lemma sup_inf_sdiff (l m : Lindenbaum T) : l * m + l * m⁻¹ = l :=
+private lemma sup_inf_sdiff (l m : Lindenbaum T) : l ⊓ m ⊔ l ⊓ mᶜ = l :=
 by { induction l using fopl.Lindenbaum.ind_on, induction m using fopl.Lindenbaum.ind_on,
-      simp[has_le.le, has_add.add, has_mul.mul, has_inv.inv, has_one.one, form.or],
+      simp[Lindenbaum.of_eq_of, has_le.le, has_sup.sup, has_inf.inf, has_compl.compl, has_top.top, form.or],
       refine ⟨contrapose.mp (deduction.mp _), _⟩, simp,
       have : ∀ n, T+{¬̇l} ⊢̇ ¬̇(l ⩑ n),
       { refine λ n, deduction.mpr (contrapose.mpr (deduction.mp _)),
@@ -366,49 +468,38 @@ by { induction l using fopl.Lindenbaum.ind_on, induction m using fopl.Lindenbaum
       refine deduction.mp (deduction.mp _), simp, refine neg_hyp (deduction.mp _),
       refine explosion (show T+{l}+{¬̇(l ⩑ m)}+{m} ⊢̇ l ⩑ m, by simp) (by simp) }
 
-private lemma inf_inf_sdiff (l m : Lindenbaum T) : l * m * (l * m⁻¹) = 0 :=
+private lemma inf_inf_sdiff (l m : Lindenbaum T) : l ⊓ m ⊓ (l ⊓ mᶜ) = ⊥ :=
 by { induction l using fopl.Lindenbaum.ind_on, induction m using fopl.Lindenbaum.ind_on,
-     simp[has_le.le, has_add.add, has_mul.mul, has_inv.inv, has_zero.zero, form.or],
+     simp[Lindenbaum.of_eq_of, has_le.le, has_sup.sup, has_inf.inf, has_compl.compl, has_bot.bot, form.or],
      refine deduction.mp (explosion (show T+{l ⩑ m ⩑ (l ⩑ ¬̇m)} ⊢̇ m, by simp[axiom_and]) (by simp[axiom_and])) }
 
-private lemma inf_compl_le_bot (l : Lindenbaum T) : l * l⁻¹ ≤ 0 :=
-by { induction l using fopl.Lindenbaum.ind_on, simp[has_le.le, has_mul.mul, has_inv.inv, has_zero.zero],
+private lemma inf_compl_le_bot (l : Lindenbaum T) : l ⊓ lᶜ ≤ ⊥ :=
+by { induction l using fopl.Lindenbaum.ind_on, simp[has_le.le, has_inf.inf, has_compl.compl, has_bot.bot],
      have : T+{l ⩑ ¬̇l} ⊢̇ l ⩑ ¬̇l, simp[-provable.and], simp at this,
      refine provable.deduction.mp (provable.explosion this.1 this.2) }
 
-private lemma top_le_sup_compl (l : Lindenbaum T) : 1 ≤ l + l⁻¹ :=
-by induction l using fopl.Lindenbaum.ind_on; simp[has_le.le, has_add.add, has_inv.inv, has_one.one, form.or]
+private lemma top_le_sup_compl (l : Lindenbaum T) : ⊤ ≤ l ⊔ lᶜ :=
+by induction l using fopl.Lindenbaum.ind_on; simp[has_le.le, has_sup.sup, has_compl.compl, has_top.top, form.or]
 
 instance : boolean_algebra (Lindenbaum T) :=
-{ bot := 0,
-  top := 1,
+{ bot := ⊥,
+  top := ⊤,
   le  := (≤),
   lt  := (<),
-  sup := (+),
-  inf := (*),
-  compl := (λ l, l⁻¹),
-  sdiff := (λ l m, l * m⁻¹),
+  sup := (⊔),
+  inf := (⊓),
+  compl := (λ l, lᶜ),
+  sdiff := (λ l m, l ⊓ mᶜ),
   le_refl := λ l, by induction l using fopl.Lindenbaum.ind_on; simp[has_le.le],
-  le_trans := λ l m n,
-  by { induction l using fopl.Lindenbaum.ind_on,
-       induction m using fopl.Lindenbaum.ind_on,
-       induction n using fopl.Lindenbaum.ind_on, simp[has_le.le], refine provable.imp_trans },
-  lt_iff_le_not_le := λ l m,
-  by { induction l using fopl.Lindenbaum.ind_on,
-       induction m using fopl.Lindenbaum.ind_on, simp[has_le.le, has_lt.lt] },
+  le_trans := λ _ _ _, le_trans,
+  lt_iff_le_not_le := λ _ _, by simp[has_lt.lt],
   le_antisymm := λ l m, le_antisymm,
   bot_le := zero_minimum,
-  le_sup_left := λ l m, by { induction l using fopl.Lindenbaum.ind_on, induction m using fopl.Lindenbaum.ind_on,
-     simp[has_add.add, has_le.le, preorder.le, provable.or_l] },
-  le_sup_right := λ l m, by { induction l using fopl.Lindenbaum.ind_on, induction m using fopl.Lindenbaum.ind_on,
-     simp[has_add.add, has_le.le, preorder.le, provable.or_r] },
+  le_sup_left := add_le_l,
+  le_sup_right := add_le_r,
   sup_le := λ _ _ _, sup_le,
-  inf_le_left := λ l m, by { induction l using fopl.Lindenbaum.ind_on,
-    induction m using fopl.Lindenbaum.ind_on, simp[has_le.le, has_mul.mul, preorder.le],
-    refine provable.hyp_and_left (by simp) },
-  inf_le_right := λ l m, by { induction l using fopl.Lindenbaum.ind_on,
-    induction m using fopl.Lindenbaum.ind_on, simp[has_le.le, has_mul.mul, preorder.le],
-    refine provable.hyp_and_right (by simp) },
+  inf_le_left := mul_le_l,
+  inf_le_right := mul_le_r,
   le_inf := λ _ _ _, le_inf,
   le_sup_inf := λ _ _ _, le_sup_inf,
   sup_inf_sdiff := sup_inf_sdiff,
@@ -417,6 +508,34 @@ instance : boolean_algebra (Lindenbaum T) :=
   inf_compl_le_bot := inf_compl_le_bot,
   top_le_sup_compl := top_le_sup_compl,
   sdiff_eq := λ _ _, rfl }
+
+theorem provable_top_iff {p} : T ⊢̇ p ↔ ⊤ ≤ ⟦p⟧ᴸ.T := iff.symm Box_iff
+
+protected theorem provable_iff {p q} : T ⊢̇ p ↔̇ q ↔ ⟦p⟧ᴸ.T = ⟦q⟧ᴸ.T := by simp[Lindenbaum.of_eq_of]
+
+theorem provable_imp_iff {p q} : T ⊢̇ p →̇ q ↔ ⟦p⟧ᴸ.T ≤ ⟦q⟧ᴸ.T := by simp[has_le.le]
+
+@[simp] lemma provable_top_eq : ⟦⊤̇⟧ᴸ.T = ⊤ := rfl
+@[simp] lemma provable_bot_eq : ⟦⊥̇⟧ᴸ.T = ⊥ := rfl
+@[simp] theorem provable_and_eq {p q} : ⟦p ⩑ q⟧ᴸ.T = ⟦p⟧ᴸ.T ⊓ ⟦q⟧ᴸ.T  := rfl
+@[simp] theorem provable_or_eq {p q} : ⟦p ⩒ q⟧ᴸ.T = ⟦p⟧ᴸ.T ⊔ ⟦q⟧ᴸ.T  := rfl
+@[simp] theorem provable_neg_eq {p} : ⟦¬̇p⟧ᴸ.T = (⟦p⟧ᴸ.T)ᶜ := rfl
+@[simp] theorem imp_eq {p q} : ⟦p →̇ q⟧ᴸ.T = (⟦p⟧ᴸ.T)ᶜ ⊔ ⟦q⟧ᴸ.T := by {
+  have : ⟦p →̇ q⟧ᴸ.T = ⟦¬̇p ⩒ q⟧ᴸ.T, 
+  { simp[Lindenbaum.of_eq_of, -provable_or_eq, form.or], refine ⟨deduction.mp (by simp), deduction.mp _⟩,
+    have : T+{¬̇¬̇p →̇ q} ⊢̇ ¬̇¬̇p →̇ q, simp[-dn1_iff], simp* at* },
+  simp[this] }
+@[simp] theorem provable_fal_eq {p} : ⟦Ȧp⟧ᴸ.T = ∏⟦p⟧ᴸ := rfl
+@[simp] theorem provable_ex_eq {p} : ⟦Ėp⟧ᴸ.T = ∐⟦p⟧ᴸ := rfl
+@[simp] lemma provable_equal_eq {t₁ t₂} : ⟦t₁ =̇ t₂⟧ᴸ.T = ⟦t₁⟧ᴴ.T ⋈ ⟦t₂⟧ᴴ.T := rfl
+@[simp] theorem provable_predicate₁_iff {p : L.pr 1} {t} : ⟦form.app p t⟧ᴸ.T = predicate₁ T p ⟦t⟧ᴴ := rfl 
+@[simp] theorem provable_predicate₂_iff {p : L.pr 2} {t₁ t₂} :
+  ⟦form.app p (vecterm.cons t₁ t₂)⟧ᴸ.T = predicate₂ T p ⟦t₁⟧ᴴ ⟦t₂⟧ᴴ := rfl 
+lemma to_Herbrand {h₁ h₂ : Herbrand T} : h₁ ⋈ h₂ = ⊤ ↔ h₁ = h₂ :=
+by { induction h₁ using fopl.Herbrand.ind_on, induction h₂ using fopl.Herbrand.ind_on,
+     simp only [equal, Herbrand.of_eq_of, has_top.top],
+     simp[-provable_equal_eq, -provable_top_eq, Lindenbaum.of_eq_of] }
+
 
 end Lindenbaum
 
